Optimizations/CanonicalizationTreeProofs.thy
@@ -6,51 +6,181 @@ theory CanonicalizationTreeProofs
     Semantics.IRTreeEvalThms
 begin
 
-lemma valid32or64:
-  assumes "valid_value (IntegerStamp b lo hi) x"
-  shows "(\<exists> v1. (x = IntVal32 v1)) \<or> (\<exists> v2. (x = IntVal64 v2))"
-  using valid32 valid64 assms valid_value.elims(2) by blast
+lemma mul_rewrite_helper:
+  shows "valid_value (IntegerStamp 32 lo hi) x \<Longrightarrow> intval_mul x (IntVal32 (-1)) = intval_negate x" 
+  and "valid_value (IntegerStamp 64 lo hi) x \<Longrightarrow> intval_mul x (IntVal64 (-1)) = intval_negate x" 
+  using valid32or64_both  by fastforce+ 
 
-lemma valid32or64_both:
-  assumes "valid_value (IntegerStamp b lox hix) x"
-  and "valid_value (IntegerStamp b loy hiy) y"
-  shows "(\<exists> v1 v2. x = IntVal32 v1 \<and> y = IntVal32 v2) \<or> (\<exists> v3 v4. x = IntVal64 v3 \<and> y = IntVal64 v4)"
-  using assms valid32or64 valid32 valid_value.elims(2) valid_value.simps(1) by metis
-
-(* -(-x) = x *)
-lemma double_negate_refinement:
-  assumes "[m,p] \<turnstile> expr \<mapsto> val"
-  assumes "stamp_expr expr = IntegerStamp b lo hi"
-  shows "(UnaryExpr UnaryNeg (UnaryExpr UnaryNeg (expr))) \<le> expr"
-proof -
-  have "valid_value (IntegerStamp b lo hi) val"
-    by (metis assms int_stamp_implies_valid_value)
-  moreover have "x = intval_negate (intval_negate x)" if "valid_value (IntegerStamp b lo hi) x" for x
-    using valid32or64 that by fastforce
-  ultimately show ?thesis using assms by (auto; (metis int_stamp_implies_valid_value)+)
+lemma CanonicalizeMulProof:
+  assumes "CanonicalizeMul before after"
+  assumes "[m, p] \<turnstile> before \<mapsto> res"
+  assumes "[m, p] \<turnstile> after \<mapsto> res'"
+  shows "res = res'"
+  using assms
+proof (induct rule: CanonicalizeMul.induct)
+  case (mul_negate32 y x lo hi)
+  then show ?case 
+    using ConstantExprE BinaryExprE bin_eval.simps evalDet mul_rewrite_helper 
+      int_stamp_implies_valid_value 
+    by (auto; metis)
+next
+  case (mul_negate64 y x lo hi)
+  then show ?case 
+    using ConstantExprE BinaryExprE bin_eval.simps evalDet mul_rewrite_helper 
+      int_stamp_implies_valid_value
+    by (auto; metis)
 qed
 
+(* (x - y) + y \<Rightarrow> x *)
+(*  x + (y - x) \<Rightarrow> y *)
+(* (-x + y) \<Rightarrow> (y - x) *)
+(* (x + (-y)) \<Rightarrow> (x - y) *)
+lemma add_rewrites_helper:
+  assumes "valid_value (IntegerStamp b lox hix) x"
+  and     "valid_value (IntegerStamp b loy hiy) y"
+
+  shows "intval_add (intval_sub x y) y = x"
+  and   "intval_add x (intval_sub y x) = y"
+  and   "intval_add (intval_negate x) y = intval_sub y x" 
+  and   "intval_add x (intval_negate y) = intval_sub x y"
+  using valid32or64_both assms by fastforce+
+
+lemma CanonicalizeAddProof:
+  assumes "CanonicalizeAdd before after"
+  assumes "[m, p] \<turnstile> before \<mapsto> res"
+  assumes "[m, p] \<turnstile> after \<mapsto> res'"
+  shows "res = res'"
+  using assms
+proof (induct rule: CanonicalizeAdd.induct)
+  case (add_xsub x a y stampa stampy)
+  then show ?case 
+    by (metis BinaryExprE Stamp.collapse(1) bin_eval.simps(1) bin_eval.simps(3) 
+        evalDet int_stamp_implies_valid_value intval_add_sym add_rewrites_helper(1))
+next
+  case (add_ysub y a x stampa stampx)
+  then show ?case 
+    by (metis is_IntegerStamp_def add_ysub.hyps add_ysub.prems evalDet BinaryExprE Stamp.sel(1) 
+        bin_eval.simps(1) bin_eval.simps(3) int_stamp_implies_valid_value intval_add_sym add_rewrites_helper(2))
+next
+  case (add_xnegate nx x stampx stampy y)
+  then show ?case 
+    by (smt (verit, del_insts) BinaryExprE Stamp.sel(1) UnaryExprE add_rewrites_helper(4) 
+        bin_eval.simps(1) bin_eval.simps(3) evalDet int_stamp_implies_valid_value intval_add_sym is_IntegerStamp_def unary_eval.simps(2))
+next
+  case (add_ynegate ny y stampx x stampy)
+  then show ?case 
+    by (smt (verit) BinaryExprE Stamp.sel(1) UnaryExprE add_rewrites_helper(4) bin_eval.simps(1) 
+        bin_eval.simps(3) evalDet int_stamp_implies_valid_value is_IntegerStamp_def unary_eval.simps(2))
+qed
+
+(* (x + y) - y \<Rightarrow> x *)
+(* (x + y) - x \<Rightarrow> y *)
+(* (x - y) - x \<Rightarrow> (-y) *)
+(* x - (x + y) \<Rightarrow> (-y) *)
+(* y - (x + y) \<Rightarrow> (-x) *)
+(* x - (x - y) \<Rightarrow> y *)
+(* x - (-y) \<Rightarrow> x + y *)
+lemma sub_rewrites_helper:
+  assumes "valid_value (IntegerStamp b lox hix) x"
+  and     "valid_value (IntegerStamp b loy hiy) y"
+
+  shows "intval_sub (intval_add x y) y  = x"
+  and   "intval_sub (intval_add x y) x  = y" 
+  and   "intval_sub (intval_sub x y) x  = intval_negate y" 
+  and   "intval_sub x (intval_add x y)  = intval_negate y"
+  and   "intval_sub y (intval_add x y)  = intval_negate x" 
+  and   "intval_sub x (intval_sub x y)  = y"
+  and   "intval_sub x (intval_negate y) = intval_add x y"
+  using valid32or64_both assms by fastforce+
+
+(* x - x \<Rightarrow> 0 *)
+(* 0 - x \<Rightarrow> -x *)
+lemma sub_single_rewrites_helper:
+  assumes "valid_value (IntegerStamp b lox hix) x"
+  shows   "b = 32 \<Longrightarrow> intval_sub x x = IntVal32 0" 
+  and     "b = 64 \<Longrightarrow> intval_sub x x = IntVal64 0"
+  and     "b = 32 \<Longrightarrow> intval_sub (IntVal32 0) x = intval_negate x" 
+  and     "b = 64 \<Longrightarrow> intval_sub (IntVal64 0) x = intval_negate x"
+  using valid32or64_both assms by fastforce+
+
+lemma CanonicalizeSubProof:
+  assumes "CanonicalizeSub before after"
+  assumes "[m, p] \<turnstile> before \<mapsto> res"
+  assumes "[m, p] \<turnstile> after \<mapsto> res'"
+  shows "res = res'"
+  using assms
+proof (induct rule: CanonicalizeSub.induct)
+  case (sub_same32 stampx x lo hi)
+  show ?case     
+    using ConstantExprE BinaryExprE  bin_eval.simps evalDet sub_same32.prems sub_single_rewrites_helper 
+      int_stamp_implies_valid_value sub_same32.hyps(1) sub_same32.hyps(2)
+    by (auto; metis)
+next
+  case (sub_same64 stampx x lo hi)
+  show ?case     
+    using ConstantExprE BinaryExprE  bin_eval.simps evalDet sub_same64.prems sub_single_rewrites_helper 
+      int_stamp_implies_valid_value sub_same64.hyps(1) sub_same64.hyps(2)
+    by (auto; metis)
+next
+  case (sub_left_add1 x a b stampa stampb)
+  then show ?case
+    by (metis BinaryExprE Stamp.collapse(1) bin_eval.simps(1) bin_eval.simps(3) evalDet 
+        int_stamp_implies_valid_value sub_rewrites_helper(1))
+next
+  case (sub_left_add2 x a b stampa stampb)
+  then show ?case
+    by (metis BinaryExprE Stamp.collapse(1) bin_eval.simps(1) bin_eval.simps(3) evalDet 
+        int_stamp_implies_valid_value sub_rewrites_helper(2))
+next
+  case (sub_left_sub x a b stampa stampb)
+  then show ?case
+    by (smt (verit) BinaryExprE Stamp.sel(1) UnaryExprE bin_eval.simps(3) evalDet
+        int_stamp_implies_valid_value is_IntegerStamp_def sub_rewrites_helper(3) unary_eval.simps(2))
+next
+  case (sub_right_add1 y a b stampa stampb)
+  then show ?case
+    by (smt (verit) BinaryExprE Stamp.sel(1) UnaryExprE bin_eval.simps(1) bin_eval.simps(3) evalDet
+        int_stamp_implies_valid_value is_IntegerStamp_def sub_rewrites_helper(4) unary_eval.simps(2))
+next
+  case (sub_right_add2 y a b stampa stampb)
+  then show ?case
+    by (smt (verit) BinaryExprE Stamp.sel(1) UnaryExprE bin_eval.simps(1) bin_eval.simps(3) evalDet
+        int_stamp_implies_valid_value is_IntegerStamp_def sub_rewrites_helper(5) unary_eval.simps(2))
+next
+  case (sub_right_sub y a b stampa stampb)
+  then show ?case
+    by (metis BinaryExprE Stamp.sel(1) bin_eval.simps(3) evalDet
+        int_stamp_implies_valid_value is_IntegerStamp_def sub_rewrites_helper(6))
+next
+  case (sub_xzero32 stampx x lo hi)
+  then show ?case     
+    using ConstantExprE BinaryExprE  bin_eval.simps evalDet sub_xzero32.prems sub_single_rewrites_helper 
+      int_stamp_implies_valid_value sub_xzero32.hyps(1) sub_xzero32.hyps(2)
+    by (auto; metis)
+next
+  case (sub_xzero64 stampx x lo hi)
+  then show ?case     
+    using ConstantExprE BinaryExprE  bin_eval.simps evalDet sub_xzero64.prems sub_single_rewrites_helper 
+      int_stamp_implies_valid_value sub_xzero64.hyps(1) sub_xzero64.hyps(2)
+    by (auto; metis)
+next
+  case (sub_y_negate nb b stampa a stampb)
+  then show ?case
+    by (smt (verit, best) BinaryExprE Stamp.sel(1) UnaryExprE bin_eval.simps(1) bin_eval.simps(3) evalDet
+        int_stamp_implies_valid_value is_IntegerStamp_def sub_rewrites_helper(7) unary_eval.simps(2))
+qed
 
 (* -(x-y) = (x-y) *)
 lemma negate_xsuby_helper:
   assumes "valid_value (IntegerStamp b lox hix) x"
   and "valid_value (IntegerStamp b loy hiy) y"
   shows "intval_negate (intval_sub x y) = intval_sub y x"
-proof -
-  have "(\<exists> v1 v2. x = IntVal32 v1 \<and> y = IntVal32 v2) \<or> (\<exists> v3 v4. x = IntVal64 v3 \<and> y = IntVal64 v4)"
-    using valid32or64_both assms by auto
-  thus ?thesis by auto
-qed
-
-lemma neg_sub_refinement:
-  assumes "[m,p] \<turnstile> x \<mapsto> xval"
-  assumes "[m,p] \<turnstile> y \<mapsto> yval"
-  assumes "stamp_expr x = IntegerStamp b lox hix"
-  assumes "stamp_expr y = IntegerStamp b loy hiy"
-  shows "(UnaryExpr UnaryNeg (BinaryExpr BinSub x y)) \<le> (BinaryExpr BinSub y x)"
-  unfolding le_expr_def
-  by (smt (verit, ccfv_threshold) assms negate_xsuby_helper int_stamp_implies_valid_value
-        evaltree.simps BinaryExprE UnaryExprE bin_eval.simps(3) unary_eval.simps(6))
+  using valid32or64_both assms by fastforce
+(* -(-x) = x *)
+lemma negate_negate_helper:
+  assumes "valid_value (IntegerStamp b lox hix) x"
+  shows "intval_negate (intval_negate x) = x" 
+  using valid32or64 assms by fastforce
 
 lemma CanonicalizeNegateProof:
   assumes "CanonicalizeNegate before after"
@@ -60,13 +190,149 @@ lemma CanonicalizeNegateProof:
   using assms
 proof (induct rule: CanonicalizeNegate.induct)
   case (negate_negate nx x)
-  thus ?case using double_negate_refinement
-    by (metis evalDet is_IntegerStamp_def le_expr_def negate_negate.hyps(1) negate_negate.prems(1) negate_negate.prems(2))
+  thus ?case 
+    by (metis UnaryExprE evalDet int_stamp_implies_valid_value is_IntegerStamp_def negate_negate_helper unary_eval.simps(2))
 next
   case (negate_sub e x y stampx stampy)
   thus ?case
-    using assms neg_sub_refinement le_expr_def evalDet is_IntegerStamp_def negate_sub.hyps negate_sub.prems
-    by (smt (verit, ccfv_SIG) BinaryExprE Stamp.collapse(1))
+    by (smt (verit) BinaryExprE Stamp.sel(1) UnaryExprE bin_eval.simps(3) evalDet int_stamp_implies_valid_value
+        is_IntegerStamp_def negate_xsuby_helper unary_eval.simps(2))
+qed
+
+(* TODO: move to values? and prove it somehow :\ *)
+lemma abs_helper:
+  assumes "\<exists> v1. x = IntVal32 (v1)"
+  shows "v1 <s 0 \<Longrightarrow> intval_abs x = IntVal32 (-v1)" 
+  and   "\<not>(v1 <s 0) \<Longrightarrow> intval_abs x = IntVal32 (v1)" 
+  using assms
+  sorry
+lemma abs_helper2:
+  assumes "\<exists> v1. x = IntVal64 (v1)"
+  shows "v1 <s 0 \<Longrightarrow> intval_abs x = IntVal64 (-v1)" 
+  and   "\<not>(v1 <s 0) \<Longrightarrow> intval_abs x = IntVal64 (v1)" 
+  using assms
+  sorry
+
+(* abs(-x) = abs(x) *)
+(* abs(abs(x)) = abs(x) *)
+lemma abs_rewrite_helper:
+  assumes "valid_value (IntegerStamp b lox hix) x"
+  shows "intval_abs (intval_negate x) = intval_abs x"
+  and "intval_abs (intval_abs x) = intval_abs x"
+  apply (metis (no_types, hide_lams) valid32or64 assms abs_helper abs_helper2
+      intval_negate.simps(1) intval_negate.simps(2))
+  by (metis valid32or64 assms abs_helper abs_helper2)
+
+lemma CanonicalizeAbsProof:
+  assumes "CanonicalizeAbs before after"
+  assumes "[m, p] \<turnstile> before \<mapsto> res"
+  assumes "[m, p] \<turnstile> after \<mapsto> res'"
+  shows "res = res'"
+  using assms
+proof (induct rule: CanonicalizeAbs.induct)
+  case (abs_abs ax x)
+  then show ?case
+    by (metis UnaryExprE abs_rewrite_helper(2) evalDet int_stamp_implies_valid_value is_IntegerStamp_def
+        unary_eval.simps(1))
+next
+  case (abs_neg nx x)
+  then show ?case
+    by (metis UnaryExprE abs_rewrite_helper(1) evalDet int_stamp_implies_valid_value is_IntegerStamp_def
+        unary_eval.simps(1) unary_eval.simps(2))
+qed
+
+(* ~(~x) = x *)
+lemma not_rewrite_helper:
+  assumes "valid_value (IntegerStamp b lox hix) x"
+  shows "intval_not (intval_not x) = x"
+  using valid32or64 assms by fastforce+
+
+lemma CanonicalizeNotProof:
+  assumes "CanonicalizeNot before after"
+  assumes "[m, p] \<turnstile> before \<mapsto> res"
+  assumes "[m, p] \<turnstile> after \<mapsto> res'"
+  shows "res = res'"
+  using assms
+proof (induct rule: CanonicalizeNot.induct)
+  case (not_not nx x)
+  then show ?case
+    by (metis UnaryExprE evalDet is_IntegerStamp_def not_rewrite_helper
+        int_stamp_implies_valid_value unary_eval.simps(3))
+qed
+
+lemma demorgans_rewrites_helper:
+  assumes "valid_value (IntegerStamp b lox hix) x"
+  and     "valid_value (IntegerStamp b loy hiy) y"
+
+  shows "intval_and (intval_not x) (intval_not y) = intval_not (intval_or x y)"
+  and   "intval_or (intval_not x) (intval_not y) = intval_not (intval_and x y)"
+  and   "x = y \<Longrightarrow> intval_and x y = x"
+  and   "x = y \<Longrightarrow> intval_or x y = x"
+  using valid32or64_both assms by fastforce+
+
+lemma CanonicalizeAndProof:
+  assumes "CanonicalizeAnd before after"
+  assumes "[m, p] \<turnstile> before \<mapsto> res"
+  assumes "[m, p] \<turnstile> after \<mapsto> res'"
+  shows "res = res'"
+  using assms
+proof (induct rule: CanonicalizeAnd.induct)
+  case (and_same x)
+  then show ?case
+    by (metis BinaryExprE bin_eval.simps(4) demorgans_rewrites_helper(3) evalDet
+        int_stamp_implies_valid_value is_IntegerStamp_def)
+next
+  case (and_demorgans nx x ny y stampx stampy)
+  then show ?case
+    by (smt (z3) BinaryExprE Stamp.sel(1) UnaryExprE bin_eval.simps(4) bin_eval.simps(5) 
+        demorgans_rewrites_helper(1) evalDet int_stamp_implies_valid_value is_IntegerStamp_def unary_eval.simps(3))
+qed
+
+lemma CanonicalizeOrProof:
+  assumes "CanonicalizeOr before after"
+  assumes "[m, p] \<turnstile> before \<mapsto> res"
+  assumes "[m, p] \<turnstile> after \<mapsto> res'"
+  shows "res = res'"
+  using assms
+proof (induct rule: CanonicalizeOr.induct)
+  case (or_same x)
+  then show ?case
+    by (metis BinaryExprE bin_eval.simps(5) demorgans_rewrites_helper(4) evalDet
+        int_stamp_implies_valid_value is_IntegerStamp_def)
+next
+  case (or_demorgans nx x ny y stampx stampy)
+  then show ?case
+    by (smt (z3) BinaryExprE Stamp.sel(1) UnaryExprE bin_eval.simps(4) bin_eval.simps(5) demorgans_rewrites_helper(2)
+        evalDet int_stamp_implies_valid_value is_IntegerStamp_def unary_eval.simps(3))
+qed
+
+lemma CanonicalizeConditionalProof:
+  assumes "CanonicalizeConditional before after"
+  assumes "[m, p] \<turnstile> before \<mapsto> res"
+  assumes "[m, p] \<turnstile> after \<mapsto> res'"
+  shows "res = res'"
+  using assms
+proof (induct rule: CanonicalizeConditional.induct)
+case (eq_branches t f c)
+  then show ?case using evalDet by auto
+next
+  case (cond_eq c x y stampx stampy)
+  then show ?case using evalDet sorry
+next
+  case (condition_bounds_x c x y stamp_x stamp_y)
+  then show ?case sorry
+next
+  case (condition_bounds_y c x y stamp_x stamp_y)
+  then show ?case sorry
+next
+  case (negate_condition nc c stampc lo hi x y)
+  then show ?case sorry
+next
+  case (const_true c val t f)
+  then show ?case using evalDet by auto
+next
+  case (const_false c val t f)
+  then show ?case using evalDet by auto
 qed
 
 end
